Manual/Releases/v4_25_1.lean
@@ -1,0 +1,23 @@
+/-
+Copyright (c) 2025 Lean FRO LLC. All rights reserved.
+Released under Apache 2.0 license as described in the file LICENSE.
+Author: Kim Morrison
+-/
+
+import VersoManual
+
+import Manual.Meta.Markdown
+
+open Manual
+open Verso.Genre
+
+
+#doc (Manual) "Lean 4.25.1 (2025-11-18)" =>
+%%%
+tag := "release-v4.25.1"
+file := "v4.25.1"
+%%%
+
+```markdown
+Lean `v4.25.1` is a bug fix release fixing a caching problem in `lake`, affecting certain downstream dependencies of `ProofWidgets4`.
+```
